cleanup examples

Fettuccine/Examples.lean
@@ -2,15 +2,9 @@ import Fettuccine.CMonomialOrder
 import Fettuccine.CMvPolynomial
 import Fettuccine.Repr
 
-abbrev σ := Fin 3
+namespace Examples
 
-section
--- Checking that the order on `Fin n` is the natural one; e.g. 0 < 1 < 2.
-example : (0 : Fin 3) < (1 : Fin 3) := by
-  decide
-example : (1 : Fin 3) < (2 : Fin 3) := by
-  decide
-end
+abbrev σ := Fin 3
 
 instance : Repr σ where
   reprPrec i _ := match i with
@@ -18,65 +12,51 @@ instance : Repr σ where
     | 1 => "y"
     | 0 => "z"
 
-namespace Examples_MvPolynomial
+namespace MvPolynomial
 
 open CMvPolynomial
+
+instance : CMonomialOrder σ := CMonomialOrder.lex
 
 def x : CMvPolynomial σ Int := X 2
 def y : CMvPolynomial σ Int := X 1
 def z : CMvPolynomial σ Int := X 0
-
 def f₁ := 3*x^2 + 2*y^3 + 3*z + 1
 def f₂ := 2*x^2 + 1*y^3 + 4*z
 def f₃ := x^2*y^3 + 2*x*y^2 + 3*z^2 + 1
 
-section
-instance : CMonomialOrder σ := CMonomialOrder.lex
 #eval f₁
-#eval f₁.leadingMonomial
 #eval f₁ + f₂
-#eval (f₁ + f₂).leadingMonomial
 #eval f₁ * f₂ * f₃
-#eval (f₁ * f₂ * f₃).leadingMonomial
-end
 
-section
-instance : CMonomialOrder σ := CMonomialOrder.grlex
-#eval f₁ + f₂
-#eval (f₁ + f₂).leadingMonomial
-#eval f₁ * f₂ * f₃
-#eval (f₁ * f₂ * f₃).leadingMonomial
-end
-
+-- We can also compute with polynomials.
 example : 3*x^2 ≠ 0 ∧ 2*y^3 ≠ 0 ∧ 3*z + 1 ≠ 0 ∧ 1 ≠ 0 := by
-  decide
+  decide -- native_decide, for ℚ.
 
--- example : 3*x^2 ≠ 0 ∧ 2*y^3 ≠ 0 ∧ 3*z + 1 ≠ 0 ∧ 1 ≠ 0 := by
---   native_decide
+end MvPolynomial
 
-end Examples_MvPolynomial
+namespace MonomialOrder
 
-namespace Examples_MonomialOrder
-
-open CMonomial CMonomialOrder
+open CMonomial
 
 def x : CMonomial σ := X 2
 def y : CMonomial σ := X 1
 def z : CMonomial σ := X 0
 
-def x2 := 2 • x
-def y3 := 3 • y
+-- To be compatible with the underlying implementation, monomials are written
+-- additively despite convention.
+def x2 := 2 • x -- x²
+def y3 := 3 • y -- y³
 def xy := x + y -- xy
 def yz := y + z -- yz
 def xy2z := x + 2 • y + z -- xy²z
 
-#eval x2
-#eval xy
-#eval yz
-#eval xy2z
-
 example : xy + x = y + x2 := by
   decide
+
+-- Let's bring in special syntax for monomial orders.
+open CMonomialOrder
+open scoped CMonomialOrder
 
 example : (x ≺[lex] x2) ∧ (xy ≺[lex] x2) ∧ (yz ≺[lex] xy)
     ∧ (xy ≺[lex] x2) ∧ (xy ≺[lex] x2 + y) := by
@@ -85,16 +65,27 @@ example : (x ≺[lex] x2) ∧ (xy ≺[lex] x2) ∧ (yz ≺[lex] xy)
 example : (x2 ≼[lex] x2) ∧ (yz ≼[lex] x2) := by
   decide
 
-example : ((x2 : CMonomial σ) ≺[grlex] y3) := by
+example : ¬(x2 ≺[lex] y3) := by
+  decide
+
+example : (x2 ≺[grlex] y3) := by
   apply grlex_isGraded -- not technically necessary... `decide` can do it too.
   decide
 
--- Can also obtain lex on `CMonomial ℕ`, if you need that.
+-- You can can also specifically name an instance in order to use it implicitly.
+section
+instance : CMonomialOrder σ := CMonomialOrder.grlex
+
+example : (x2 ≺ y3) := by
+  decide
+end
+
+-- Can also obtain lex on `CMonomial ℕ`, if you need infinite variables.
 example : CMonomialOrder ℕ := lex
 
-end Examples_MonomialOrder
+end MonomialOrder
 
-section Examples_LeadingMonomial
+namespace LeadingMonomial
 
 open CMonomialOrder CMvPolynomial
 
@@ -117,4 +108,6 @@ instance : CMonomialOrder σ := grlex
 #eval f₂.leadingMonomial
 end
 
-end Examples_LeadingMonomial
+end LeadingMonomial
+
+end Examples
